backend/Lineartyping.v
@@ -266,12 +266,12 @@ Inductive wt_state: state -> Prop :=
         (AGCS: agree_callee_save rs (parent_locset s))
         (AGARGS: agree_outgoing_arguments (funsig fd) rs (parent_locset s)),
       wt_state (Callstate s fd rs m)
-  | wt_return_state: forall s rs m sg cp
+  | wt_return_state: forall s rs m
         (WTSTK: wt_callstack s)
         (WTRS: wt_locset rs)
         (AGCS: agree_callee_save rs (parent_locset s))
         (UOUT: outgoing_undef rs),
-      wt_state (Returnstate s rs m sg cp).
+      wt_state (Returnstate s rs m).
 
 (** Preservation of state typing by transitions *)
 
@@ -453,8 +453,8 @@ Proof.
 Qed.
 
 Lemma wt_returnstate_agree:
-  forall s rs m sg cp,
-  wt_state (Returnstate s rs m sg cp) ->
+  forall s rs m,
+  wt_state (Returnstate s rs m) ->
   agree_callee_save rs (parent_locset s) /\ outgoing_undef rs.
 Proof.
   intros. inv H; auto.
